cava/monad-examples/Examples.v
@@ -14,29 +14,9 @@
 (* limitations under the License.                                           *)
 (****************************************************************************)
 
-(* A codification of the Lava embedded DSL develope for Haskell into
-   Coq for the specification, implementaiton and formal verification of
-   circuits. Experimental work, very much in flux, as Satnam learns Coq!
-*)
-
-Require Import Program.Basics.
-From Coq Require Import Bool.Bool.
-From Coq Require Import Ascii String.
-From Coq Require Import Lists.List.
-From Coq Require Import NArith.
-Import ListNotations.
-
-Require Import ExtLib.Structures.Monads.
-Export MonadNotation.
-Open Scope monad_scope.
+(* Experiments with the primitives that form the core of Cava. *)
 
 Require Import Cava.Monad.Cava.
-Require Import Cava.Monad.Combinators.
-Require Import Cava.Netlist.
-Require Import Cava.BitArithmetic.
-
-Local Open Scope list_scope.
-Local Open Scope monad_scope.
 
 (* Experiments with the primitive Cava gates. *)
 
@@ -51,88 +31,3 @@ Proof. reflexivity. Qed.
 
 Example and_11 : combinational (and2 (true, true)) = true.
 Proof. reflexivity. Qed.
-
-(* Unsigned addition examples. *)
-
-Definition bv4_0  := nat_to_bitvec_sized 4  0.
-Definition bv4_1  := nat_to_bitvec_sized 4  1.
-Definition bv4_2  := nat_to_bitvec_sized 4  2.
-Definition bv4_3  := nat_to_bitvec_sized 4  3.
-Definition bv4_15 := nat_to_bitvec_sized 4 15.
-
-Definition bv5_0  := nat_to_bitvec_sized 5  0.
-Definition bv5_3  := nat_to_bitvec_sized 5  3.
-Definition bv5_16 := nat_to_bitvec_sized 5 16.
-Definition bv5_30 := nat_to_bitvec_sized 5 30.
-
-(* Check 0 + 0 = 0 *)
-Example add_0_0 : combinational (unsignedAdd bv4_0 bv4_0) = bv5_0.
-Proof. reflexivity. Qed.
-
-(* Check 1 + 2 = 3 *)
-Example add_1_2 : combinational (unsignedAdd bv4_1 bv4_2) = bv5_3.
-Proof. reflexivity. Qed.
-
-(* Check 15 + 1 = 16 *)
-Example add_15_1 : combinational (unsignedAdd bv4_15 bv4_1) = bv5_16.
-Proof. reflexivity. Qed.
-
-(* Check 15 + 15 = 30 *)
-Example add_15_15 : combinational (unsignedAdd bv4_15 bv4_15) = bv5_30.
-Proof. reflexivity. Qed.
-
-(* An adder example. *)
-
-Definition adder4Top : state CavaState (Vector.t N 5) :=
-  setModuleName "adder4" ;;
-  a <- inputVectorTo0 4 "a" ;;
-  b <- inputVectorTo0 4 "b" ;;
-  sum <- unsignedAdd a b ;;
-  outputVectorTo0 5 sum "sum".
-
-Definition adder4Netlist := makeNetlist adder4Top.
-
-(* An contrived example of loopBit *)
-
-Definition loopedNAND {m bit} `{Cava m bit}  := loopBit (second delayBit >=> nand2 >=> fork2).
-
-Definition loopedNANDTop : state CavaState N :=
-  setModuleName "loopedNAND" ;;
-  a <- inputBit "a" ;;
-  b <- loopedNAND a ;;
-  outputBit "b" b.
-
-Definition loopedNANDNetlist := makeNetlist loopedNANDTop.
-
-Fixpoint loopedNAND_spec' (i : list bool) (state : bool) : list bool :=
-  match i with
-  | [] => []
-  | x::xs => let newOutput := negb (x && state) in
-             newOutput :: loopedNAND_spec' xs newOutput
-  end.
-
-(*
-Definition loopedNAND_spec (i : list bool) : list bool := loopedNAND_spec' i false.
-
-Lemma peel_list : forall (a : bool) (x y : list bool),
-                  a::x = a::y <-> x = y.
-Proof.
-  intros.
-  destruct x.
-
-
-Lemma noopedNAND_behaviour : forall (a : list bool),
-                             sequential (loopedNAND a) = loopedNAND_spec a.
-Proof.
-  intros.
-  unfold sequential.
-  unfold unIdent.
-  simpl.
-  unfold loopedNAND_spec.
-  induction a.
-  auto.
-  simpl.
-  rewrite peel_list.
-*)
-
-  
