cava/cava/Cava/Monad/UnsignedAdders.v
@@ -1,0 +1,100 @@
+(****************************************************************************)
+(* Copyright 2020 The Project Oak Authors                                   *)
+(*                                                                          *)
+(* Licensed under the Apache License, Version 2.0 (the "License")           *)
+(* you may not use this file except in compliance with the License.         *)
+(* You may obtain a copy of the License at                                  *)
+(*                                                                          *)
+(*     http://www.apache.org/licenses/LICENSE-2.0                           *)
+(*                                                                          *)
+(* Unless required by applicable law or agreed to in writing, software      *)
+(* distributed under the License is distributed on an "AS IS" BASIS,        *)
+(* WITHOUT WARRANTIES OR CONDITIONS OF ANY KIND, either express or implied. *)
+(* See the License for the specific language governing permissions and      *)
+(* limitations under the License.                                           *)
+(****************************************************************************)
+
+(* A codification of the Lava embedded DSL develope for Haskell into
+   Coq for the specification, implementaiton and formal verification of
+   circuits. Experimental work, very much in flux, as Satnam learns Coq!
+*)
+
+From Coq Require Import Vector.
+From Coq Require Import Bool.Bvector.
+
+
+Require Import ExtLib.Structures.Monads.
+Export MonadNotation.
+Open Scope monad_scope.
+
+Require Import Cava.Monad.Cava.
+Require Import Cava.Monad.Combinators.
+Require Import Cava.Netlist.
+Require Import Cava.BitArithmetic.
+
+Require Import Nat Arith Lia.
+
+
+(******************************************************************************)
+(* An adder with two inputs that must be the same length.                     *)
+(******************************************************************************)
+
+Definition adderFixed {m bit} `{Cava m bit} {inputSize : nat}
+                      (sumSize : nat)
+                      (a : (Vector.t bit inputSize))
+                      (b : (Vector.t bit inputSize))
+                      : m (Vector.t bit sumSize) :=
+  a_plus_b <- unsignedAdd sumSize a b ;;
+  ret a_plus_b.
+
+(******************************************************************************)
+(* A three input adder.                                                       *)
+(******************************************************************************)
+
+Definition adder_3input {m bit} `{Cava m bit} {inputSize : nat}
+                        (sumSize : nat)
+                        (a : (Vector.t bit inputSize))
+                        (b : (Vector.t bit inputSize))
+                        (c : (Vector.t bit inputSize))
+                        : m (Vector.t bit sumSize) :=
+  a_plus_b <- unsignedAdd sumSize a b ;;
+  sum <- unsignedAdd sumSize a_plus_b c ;;
+  ret sum.
+
+Lemma mod_plus_mod: forall a b c n, n > 0 ->
+                    ((a + b) mod n + c) mod n = (a + b + c) mod n.
+Proof.
+  intros.
+  rewrite Nat.add_mod_idemp_l.
+  - reflexivity.
+  - lia.
+Qed.
+
+Lemma two_p_gt_0: forall n, 2^n > 0.
+Proof.
+  intros.
+  induction n.
+  - simpl. lia.
+  - rewrite Nat.pow_succ_r.
+    + lia.
+    + lia.
+Qed.
+
+Lemma add3_behaviour : forall {inputSize : nat} (sumSize : nat)
+                       (av : Bvector inputSize)
+                       (bv : Bvector inputSize)
+                       (cv : Bvector inputSize),
+                       let a := bitvec_to_nat av in
+                       let b := bitvec_to_nat bv in
+                       let c := bitvec_to_nat cv in
+                       bitvec_to_nat (combinational (adder_3input sumSize av bv cv))
+                         = (a + b + c) mod 2^sumSize.
+Proof.
+  intros. unfold combinational. unfold adder_3input. simpl.
+  do 2 rewrite nat_of_bits_sized_n.
+  fold a b c.
+  rewrite mod_plus_mod.
+  - reflexivity.
+  - apply two_p_gt_0.
+Qed.
+
