cava/monad-examples/UnsignedAdderExamples.v
@@ -1,0 +1,142 @@
+(****************************************************************************)
+(* Copyright 2020 The Project Oak Authors                                   *)
+(*                                                                          *)
+(* Licensed under the Apache License, Version 2.0 (the "License")           *)
+(* you may not use this file except in compliance with the License.         *)
+(* You may obtain a copy of the License at                                  *)
+(*                                                                          *)
+(*     http://www.apache.org/licenses/LICENSE-2.0                           *)
+(*                                                                          *)
+(* Unless required by applicable law or agreed to in writing, software      *)
+(* distributed under the License is distributed on an "AS IS" BASIS,        *)
+(* WITHOUT WARRANTIES OR CONDITIONS OF ANY KIND, either express or implied. *)
+(* See the License for the specific language governing permissions and      *)
+(* limitations under the License.                                           *)
+(****************************************************************************)
+
+Require Import Program.Basics.
+From Coq Require Import Bool.Bool.
+From Coq Require Import Ascii String.
+From Coq Require Import Lists.List.
+From Coq Require Import NArith.
+Import ListNotations.
+
+Require Import ExtLib.Structures.Monads.
+Export MonadNotation.
+Open Scope monad_scope.
+
+Require Import Cava.Netlist.
+Require Import Cava.BitArithmetic.
+Require Import Cava.Monad.Cava.
+Require Import Cava.Monad.UnsignedAdders.
+
+Local Open Scope list_scope.
+Local Open Scope monad_scope.
+
+(******************************************************************************)
+(* Unsigned addition examples.                                                *)
+(******************************************************************************)
+
+Definition bv4_0  := nat_to_bitvec_sized 4  0.
+Definition bv4_1  := nat_to_bitvec_sized 4  1.
+Definition bv4_2  := nat_to_bitvec_sized 4  2.
+Definition bv4_3  := nat_to_bitvec_sized 4  3.
+Definition bv4_15 := nat_to_bitvec_sized 4 15.
+
+Definition bv5_0  := nat_to_bitvec_sized 5  0.
+Definition bv5_3  := nat_to_bitvec_sized 5  3.
+Definition bv5_16 := nat_to_bitvec_sized 5 16.
+Definition bv5_30 := nat_to_bitvec_sized 5 30.
+
+(* Check 0 + 0 = 0 *)
+Example add5_0_0 : combinational (unsignedAdd 5 bv4_0 bv4_0) = bv5_0.
+Proof. reflexivity. Qed.
+
+(* Check 1 + 2 = 3 *)
+Example add5_1_2 : combinational (unsignedAdd 5 bv4_1 bv4_2) = bv5_3.
+Proof. reflexivity. Qed.
+
+(* Check 15 + 1 = 16 *)
+Example add5_15_1 : combinational (unsignedAdd 5 bv4_15 bv4_1) = bv5_16.
+Proof. reflexivity. Qed.
+
+(* Check 15 + 1 = 16 for 4-bit result *)
+Example add4_15_1 : combinational (unsignedAdd 4 bv4_15 bv4_1)
+                  = nat_to_bitvec_sized 4 0.
+Proof. reflexivity. Qed.
+
+(* Check 15 + 15 = 30 *)
+Example add5_15_15 : combinational (unsignedAdd 5 bv4_15 bv4_15) = bv5_30.
+Proof. reflexivity. Qed.
+
+(* Check 15 + 15 = 14 for 4-bit result *)
+Example add4_15_15 : combinational (unsignedAdd 4 bv4_15 bv4_15)
+                   = nat_to_bitvec_sized 4 14.
+Proof. reflexivity. Qed.
+
+(* Check 15 + 15 = 6 for 3-bit result *)
+Example add3_15_15 : combinational (unsignedAdd 3 bv4_15 bv4_15)
+                   = nat_to_bitvec_sized 3 6.
+Proof. reflexivity. Qed.
+
+(* Check 15 + 15 = 2 for 2-bit result *)
+Example add2_15_15 : combinational (unsignedAdd 2 bv4_15 bv4_15)
+                   = nat_to_bitvec_sized 2 2.
+Proof. reflexivity. Qed.
+
+(* Check 15 + 15 = 0 for 1-bit result *)
+Example add1_15_15 : combinational (unsignedAdd 1 bv4_15 bv4_15)
+                   = nat_to_bitvec_sized 1 0.
+Proof. reflexivity. Qed.
+
+(* An adder example. *)
+
+(******************************************************************************)
+(* Generate a 4-bit unsigned adder with 5-bit output.                         *)
+(******************************************************************************)
+
+Definition adder4Top : state CavaState (Vector.t N 5) :=
+  setModuleName "adder4" ;;
+  a <- inputVectorTo0 4 "a" ;;
+  b <- inputVectorTo0 4 "b" ;;
+  sum <- unsignedAdd 5 a b ;;
+  outputVectorTo0 5 sum "sum".
+
+Definition adder4Netlist := makeNetlist adder4Top.
+
+(******************************************************************************)
+(* Generate a three input 8-bit unsigned adder with 10-bit output.            *)
+(******************************************************************************)
+
+Definition adder8_3inputTop : state CavaState (Vector.t N 10) :=
+  setModuleName "adder8_3input" ;;
+  a <- inputVectorTo0 8 "a" ;;
+  b <- inputVectorTo0 8 "b" ;;
+  c <- inputVectorTo0 8 "c" ;;
+  sum <- adder_3input 10 a b c ;;
+  outputVectorTo0 10 sum "sum".
+
+Definition adder8_3inputNetlist := makeNetlist adder8_3inputTop.
+
+(******************************************************************************)
+(* An contrived example of loopBit                                            *)
+(******************************************************************************)
+
+Definition loopedNAND {m bit} `{Cava m bit}  := loopBit (second delayBit >=> nand2 >=> fork2).
+
+Definition loopedNANDTop : state CavaState N :=
+  setModuleName "loopedNAND" ;;
+  a <- inputBit "a" ;;
+  b <- loopedNAND a ;;
+  outputBit "b" b.
+
+Definition loopedNANDNetlist := makeNetlist loopedNANDTop.
+
+Fixpoint loopedNAND_spec' (i : list bool) (state : bool) : list bool :=
+  match i with
+  | [] => []
+  | x::xs => let newOutput := negb (x && state) in
+             newOutput :: loopedNAND_spec' xs newOutput
+  end.
+
+  
